proof/correctness/Utils2.ec
@@ -134,6 +134,13 @@ pred mem_dif (m m' : global_mem_t) (p : int) = m.[p] <> m'.[p].
 (** -------------------------------------------------------------------------------------------- **)
 
 
+lemma pow2_pos (e : int) :
+    0 < e => 0 < 2^e.
+proof.
+move => H.
+admit.
+qed.
+
 lemma pow2_neq_0  (t : int) : 
     0 <= t => 0 <> 2^t by smt(@Real).
 
